Experiment with expressing semantics in terms of nat64 instead of uint. Preliminary data suggests that it leads to cleaner semantics, requires two small lemmas in decls, and generally improves proof performance time.

tools/scripts/collect-fstar-times.py
@@ -88,13 +88,14 @@ def compute_diff(times1, times2):
     return diffs
 
 def display_diffs(times, diffs):
-    tab = PrettyTable(["Filename", "t1 time", "delta", "delta \%","Full Path"])
+    delta_label = "delta: t1 - t2"
+    tab = PrettyTable(["Filename", "t1 time", delta_label, "delta \%","Full Path"])
     tab.align["Filename"] = "l"
     tab.align["t1 time"] = "r"
-    tab.align["delta"] = "r"
+    tab.align[delta_label] = "r"
     tab.align["delta \%"] = "r"
     tab.align["FullPath"] = "l"
-    tab.sortby = "delta"
+    tab.sortby = delta_label
 
     total_time = 0
     total_delta = 0
@@ -105,7 +106,7 @@ def display_diffs(times, diffs):
         delta_percent = "n/a"
         if f in diffs:
             delta = diffs[f]
-            delta_percent = "%0.1f" % (delta / float(times[f]))
+            delta_percent = "%0.1f" % (delta / float(times[f]) * 100)
         tab.add_row([filename, times[f], delta, delta_percent, f])
         if not times[f] is None:
             total_time += times[f]
